let's look at the following equation 

-2 = -2 

can be written as,

1 - 3 = 4 - 6 #step0

also as,

--> 1^2 - 3 = 2^2 - 6 #step1

add 9/4 to both sides,

--> 1^2 - 3 + 9/4 = 2^2 - 6 + 9/4 #step2

write in the form of a^2 - 2ab + b^2

--> 1^2 - 2*1*(3/2) + (3/2)^2 = 2^2 - 2*2*(3/2) + (3/2)^2 #step3

narrow to the form (a - b)^2

--> (1 - 3/2)^2 = (2 - 3/2)^2 #step4

cancel the squares from both sides

--> 1 - 3/2 = 2 - 3/2 #step5

cancel the 3/2 term

--> 1 = 2 #result

(from https://www.quora.com/How-can-you-make-1+1-1)

that seems true.
but it got a mistakes.
or there is only 1/2 chance for it to sussess.
when you move a square to another side of a equation
it will be -sqrt(something) or +sqrt(something)
look at the process from step 4 to step 5
it move the square
so there will be some possable results

1. 1 = 2 = 1 + 1  
2. -1 + 3/2 = 2 - 3/2  
  --> 3 = 3 # -(sqrt(1 - 3/2)^2)  
3. 1 - 3/2 + -2 + 3/2  
  --> 3 = 3 # -(sqrt(2 - 3/2)^2)  
